tools/coqdep.sh
@@ -1,6 +1,8 @@
-THEORIES=../../coq/theories/
+THEORIES=../../coq/
 
-modules=$(find $THEORIES -name "*.d" -exec cat '{}' ';' | python gendep.py)
+
+
+modules=$(find $THEORIES -name "*.d" -exec cat '{}' ';' | sed ':a;N;$!ba;s/\\\s*\n/ /g' | python gendep.py)
 
 echo "Require Import $modules."
 for x in $modules; do 
